complete reorg & rewrite
Signed-off-by: Alexander Diemand <codieplusplus@apax.net>

bin/lxr_assembly.ml
@@ -1,11 +1,19 @@
 (* open Lwt *)
 
-(* open Elykseer__Lxr *)
+open Elykseer__Lxr
+open Elykseer__Lxr.Buffer
 open Elykseer__Lxr.Assembly
+open Elykseer__Lxr.Configuration
+(* open Elykseer__Lxr.Conversion *)
 (* open Elykseer__Lxr.Block *)
-open Elykseer__Lxr.Environment
+(* open Elykseer__Lxr.Environment *)
 
 open Elykseer_utils
+open Elykseer_base
+
+open Mlcpp_cstdio
+open Mlcpp_chrono
+
 
 let arg_verbose = ref false
 let arg_fctrl = ref ""
@@ -20,19 +28,47 @@ let argspec =
 
 let anon_args_fun _fn = ()
 
-let assembly_check e p_aid : assembly option Lwt.t =
-    Lwt.return @@ List.find_opt (fun a -> aid a = p_aid) e.assemblies
+(* let assembly_check e p_aid : assembly option Lwt.t =
+    Lwt.return @@ List.find_opt (fun a -> aid a = p_aid) e.assemblies *)
+
+let bm_add_content content buffer sz =
+    (* let buffer = Cstdio.File.Buffer.create (16*256*1024) in *)
+    Assembly.add_content content sz 0 buffer
+
+let benchmark_add_content =
+  let msg = "testing some longer message." in
+  let content = Cstdio.File.Buffer.init (16*256*1024) (fun i -> if i < 28 then String.get msg i else '0') in
+  let clock1 = Chrono.Clock.System.now () in
+  let buffer = Cstdio.File.Buffer.create (16*256*1024) in
+  for _i = 0 to 999 do
+    let bench = bm_add_content content buffer (1*256*1024) in
+    if bench = (1*256*1024) then print_string "√" else print_char '?'
+  done;
+  let clock2 = Chrono.Clock.System.now () in
+  let tdiff = Chrono.Clock.System.diff clock2 clock1 in
+  Lwt_io.printlf "time: %s" (Chrono.Duration.to_string @@ Chrono.Duration.cast_ms tdiff)
 
 (* main *)
-let main () = Arg.parse argspec anon_args_fun "lxr_assemlby: vaf";
-    let _setup = setup_environment in
+let main () = Arg.parse argspec anon_args_fun "lxr_assembly: vaf";
+    (* let _setup = setup_environment in
     let e = Envutils.envrestore !arg_fctrl in
     let%lwt () = Lwt_io.printl (Utils.e2s e) in
-    let%lwt a = assembly_check e !arg_aid in
-    match a with
-    | None -> Lwt_io.printl "nothing found"
-    | Some a0 ->
-        let a1 = restore (e.config) a0 in
-        Lwt_io.printl (Utils.as2s a1)
+    let%lwt a = assembly_check e !arg_aid in *)
+    let c : Configuration.configuration = { path_chunks = "./chunks"; path_meta = "./meta"; my_id = Conversion.i2n 16} in
+    let (a,b) = AssemblyPlainWritable.create c (Nchunks.from_int 16) in
+    let%lwt () = Lwt_io.printf "assembly %s %d %d" a.aid (Conversion.p2i a.nchunks) (Conversion.n2i a.apos) in
+    let%lwt () = Lwt_io.printf "block size %d" (Conversion.n2i @@ AssemblyPlainWritable.buffer_len b) in
+    let%lwt () = Lwt_io.printl (Utils.as2s a) in
+    let%lwt () = Lwt_io.printlf "buffer sha256 = %s" (AssemblyPlainWritable.calc_checksum b) in
+    (* let msg = "testing some longer message." in *)
+    let content = BufferPlain.buffer_create (Conversion.i2n 1024) in (*  (fun i -> if i < 28 then String.get msg i else '0') in *)
+    let relfiles = RelationFileAid.coq_new in
+    let (a', _relfiles') = backup a b "test1M" content relfiles in
+    let relkey = (RelationAidKey.add "abc97391af" (aid a') RelationAidKey.coq_new ) in
+    let (a'', b') = Elykseer__Lxr.Assembly.finish a' b in
+    match Elykseer__Lxr.Assembly.encrypt a'' b' relkey with
+    | None -> Lwt_io.printl "failed to encrypt"
+    | Some (_a''', b'') -> Lwt_io.printlf "sha256 = %s" (AssemblyEncrypted.calc_checksum b'') |> ignore ;
+    benchmark_add_content
 
 let () = Lwt_main.run (main ())
