bin/lxr_restore.ml
@@ -1,0 +1,48 @@
+
+(* open Elykseer *)
+open Elykseer__Lxr
+open Elykseer__Lxr.Configuration
+
+let def_myid = 1234567890
+
+let arg_verbose = ref false
+let arg_files = ref []
+let arg_metapath = ref "meta"
+let arg_chunkpath = ref "lxr"
+let arg_nchunks = ref "16"
+let arg_myid = ref (string_of_int def_myid) (* "1234567890" *)
+
+let argspec =
+  [
+    ("-v", Arg.Set arg_verbose, "verbose output");
+    ("-x", Arg.Set_string arg_chunkpath, "sets path for encrypted chunks");
+    ("-f", Arg.Set_string arg_metapath, "sets path for meta data");
+    ("-n", Arg.Set_string arg_nchunks, "sets number of chunks (16-256) per assembly");
+    ("-i", Arg.Set_string arg_myid, "sets own identifier");
+  ]
+
+let anon_args_fun fn = arg_files := fn :: !arg_files
+
+let rec backup_files conf0 e0 fns =
+        match fns with
+          [] -> e0
+        | fn :: fns' -> let e1 = backup_file conf0 e0 fn in
+                        backup_files conf0 e1 fns'
+
+(* main *)
+let () = Arg.parse argspec anon_args_fun "lxr_restore: vxfni";
+         let nchunks = int_of_string !arg_nchunks in
+         if List.length !arg_files > 0 &&
+            nchunks >= 16 && nchunks <= 256
+         then
+           let _setup = setup_environment in
+           let myid = let id0 = int_of_string !arg_myid in
+                      if id0 >= 0 then id0 else def_myid in
+           let conf0 : configuration = {
+                         num_chunks  = Conversion.i2p nchunks ;
+                         path_chunks = !arg_chunkpath;
+                         path_meta   = !arg_metapath;
+                         my_id       = Conversion.i2n myid } in
+           let e0 = initial_environment conf0 in
+           let e1 = restore_file conf0 e0 !arg_files in
+           print_string @@ Elykseer_utils.Utils.e2j e1;
