elykseer-base/buffer.ml
@@ -1,0 +1,8 @@
+open Mlcpp_cstdio
+
+type b = Cstdio.File.Buffer.ta
+
+external buffer_sha_id : b -> Sha256.buf = "cpp_buffer_sha_id"
+let sha256 b =
+  let b' = buffer_sha_id b in
+  Sha256.buffer b'
