helper.cxx
@@ -1,0 +1,20 @@
+// OCaml includes
+extern "C" {
+#include <caml/mlvalues.h>
+#include <caml/memory.h>
+#include <caml/alloc.h>
+#include <caml/bigarray.h>
+#include <caml/custom.h>
+// #include <caml/callback.h>
+#include <caml/fail.h>
+
+#include <sys/errno.h>
+} //extern C
+
+
+extern "C" {
+value cpp_buffer_id(value vbuf)
+{
+    return vbuf;
+}
+} // extern C
