helper.ml
@@ -1,0 +1,26 @@
+
+external cpp_buffer_id : 'a -> 'b = "cpp_buffer_id"
+
+
+let store_chunk_to_path fp sz pos b =
+  if Mlcpp_filesystem.Filesystem.Path.exists fp
+  then 0
+  else let buf = Mlcpp_cstdio.Cstdio.File.Buffer.create sz in
+       let _n = Mlcpp_cstdio.Cstdio.File.Buffer.copy_sz_pos b pos sz buf 0 in
+       match Mlcpp_cstdio.Cstdio.File.fopen (Mlcpp_filesystem.Filesystem.Path.to_string fp) "wx" with
+       | Error _ -> 0
+       | Ok fptr -> match Mlcpp_cstdio.Cstdio.File.fwrite buf sz fptr with
+                    | Error _ -> 0
+                    | Ok cnt -> cnt
+
+let load_chunk_from_path fp =
+  let b = Mlcpp_cstdio.Cstdio.File.Buffer.create (256*1024) in
+  if Mlcpp_filesystem.Filesystem.Path.exists fp
+  then Mlcpp_cstdio.Cstdio.File.fopen (Mlcpp_filesystem.Filesystem.Path.to_string fp) "rx" |> function
+    | Error _ -> None
+    | Ok fptr -> begin
+        Mlcpp_cstdio.Cstdio.File.fread b (256*1024) fptr |> function
+        | Error _ -> None
+        | Ok _cnt -> Some b
+    end
+  else None
