test/testAssembly.ml
@@ -1,0 +1,25 @@
+open Elykseer_base
+open Mlcpp_cstdio
+
+module Testing = struct
+  let add_content = fun bsrc sz pos btgt -> Assembly.add_content bsrc sz pos btgt
+
+end
+
+(* Tests *)
+
+let test_add_content () =
+  let msg = "testing" in
+  let content = Cstdio.File.Buffer.init 32 (fun i -> if i < 7 then String.get msg i else '0') in
+  let buffer = Cstdio.File.Buffer.create (16*256*1024) in
+  Alcotest.(check int) "add content"
+  4 (* == *) (Testing.add_content content 4 0 buffer)
+
+(* Runner *)
+
+let test =
+  let open Alcotest in
+  "LXR Assembly",
+  [
+    test_case "add content" `Quick test_add_content;
+  ]
