theories/MakeML.v
@@ -1,0 +1,158 @@
+
+Require Coq.extraction.Extraction.
+Extraction Language OCaml.
+
+Require Import ZArith NArith.
+Open Scope positive_scope.
+
+From LXR Require Import Assembly.
+From LXR Require Import Buffer.
+From LXR Require Import Configuration.
+From LXR Require Import Conversion.
+From LXR Require Import RelationAidKey.
+From LXR Require Import RelationFileAid.
+From LXR Require Import Utilities.
+
+From Coq Require Import ExtrOcamlBasic.
+From Coq Require Import ExtrOcamlNativeString.
+
+
+Extract Inductive bool => "bool" [ "true" "false" ].
+Extract Inductive sumbool => "bool" ["true" "false"].
+Extract Inductive option => option [ Some None ].
+
+(** the following were found in: https://github.com/coq-contribs/zchinese 
+    and are very useful to convert standard OCaml 'int' into positive|N|Z *)
+
+Extract Inlined Constant int => "int".
+
+Extract Constant i2p =>
+   "  
+    let rec i2p = function 
+       1 -> XH 
+     | n -> let n' = i2p (n/2) in if (n mod 2)=0 then XO n' else XI n'
+     in i2p
+   ".
+ 
+Extract Constant p2i =>
+   "
+    let rec p2i = function 
+       XH -> 1
+     | XO p -> 2*(p2i p)
+     | XI p -> 2*(p2i p)+1
+     in p2i 
+   ".
+
+Extract Constant i2z =>
+   "
+    function 
+      0 -> Z0
+    | n -> if n < 0 then Zneg (i2p (-n)) else Zpos (i2p n)
+   ".
+
+Extract Constant z2i =>
+   "
+    function
+      Z0 -> 0 
+    | Zpos p -> p2i p
+    | Zneg p -> -(p2i p)
+   ".
+
+Extract Constant i2n =>
+   "
+    function 
+      0 -> N0
+    | n -> Npos (i2p n)
+   ".
+
+Extract Constant n2i =>
+   "
+    function
+      N0 -> 0 
+    | Npos p -> p2i p
+   ".
+
+Extract Constant rndsetup =>
+   "
+    function
+     _ -> Random.self_init (); Conversion.i2n 0
+   ".
+
+Extract Constant rnd =>
+   "
+    function
+     _ -> int_of_float  (2. ** 30. -. 1.) |> Random.int |> Conversion.i2n
+   ".
+
+Extract Constant rnd256 =>
+   "
+   function
+   x -> int_of_float  (2. ** 30. -. 1.) |> Random.int |> string_of_int |>
+     String.cat (Conversion.n2i x |> string_of_int) |>
+     String.cat (Unix.gethostname ()) |> String.cat (Unix.gettimeofday () |> string_of_float) |>
+     Sha256.string |> Sha256.to_hex
+   ".
+
+Extract Constant chunk_identifier =>
+   "  
+    fun config aid cid -> let s =
+      (string_of_int (Conversion.n2i (Configuration.my_id config))) ^
+      (string_of_int (Conversion.p2i cid)) ^
+      aid in
+      Printf.eprintf ""c id: %s\n"" s;
+      Elykseer_base.Hashing.sha256 s
+   ".
+
+Extract Constant chunk_identifier_path =>
+   "  
+    fun config aid cid -> let cident = chunk_identifier config aid cid in
+      (Configuration.path_chunks config ^ ""/"" ^ cident ^ "".lxr"")
+   ".
+
+Extract Constant BufferEncrypted.buffer_t => "Mlcpp_cstdio.Cstdio.File.Buffer.ta".
+Extract Constant BufferEncrypted.buffer_create => "fun n -> Mlcpp_cstdio.Cstdio.File.Buffer.create (Conversion.n2i n)".
+Extract Constant BufferEncrypted.buffer_len => "fun b -> Conversion.i2n (Mlcpp_cstdio.Cstdio.File.Buffer.size b)".
+Extract Constant BufferEncrypted.calc_checksum => "fun b -> Sha256.to_hex @@ Elykseer_base.Buffer.sha256 b".
+
+Extract Constant BufferPlain.buffer_t => "Mlcpp_cstdio.Cstdio.File.Buffer.ta".
+Extract Constant BufferPlain.buffer_create => "fun n -> Mlcpp_cstdio.Cstdio.File.Buffer.create (Conversion.n2i n)".
+Extract Constant BufferPlain.buffer_len => "fun b -> Conversion.i2n (Mlcpp_cstdio.Cstdio.File.Buffer.size b)".
+Extract Constant BufferPlain.calc_checksum => "fun b -> Sha256.to_hex @@ Elykseer_base.Buffer.sha256 b".
+
+Extract Constant id_buffer_t_from_enc => "fun b -> Helper.cpp_buffer_id b".
+Extract Constant id_buffer_t_from_full => "fun b -> Helper.cpp_buffer_id b".
+Extract Constant id_buffer_t_from_writable => "fun b -> Helper.cpp_buffer_id b".
+Extract Constant id_assembly_plain_buffer_t_from_buf => "fun b -> Helper.cpp_buffer_id b".
+Extract Constant id_assembly_enc_buffer_t_from_buf => "fun b -> Helper.cpp_buffer_id b".
+Extract Constant id_enc_from_buffer_t => "fun b -> Helper.cpp_buffer_id b".
+Extract Constant id_assembly_full_buffer_from_writable => "fun b -> Helper.cpp_buffer_id b".
+
+Extract Constant cpp_encrypt_buffer => "fun b _pw -> Helper.cpp_buffer_id b".  (* TODO *)
+Extract Constant cpp_decrypt_buffer => "fun b _pw -> Helper.cpp_buffer_id b".  (* TODO *)
+
+Extract Constant BufferEncrypted.copy_sz_pos =>
+   "
+    fun bsrc npos1 nsz btgt npos2 -> Conversion.i2n @@
+      Mlcpp_cstdio.Cstdio.File.Buffer.copy_sz_pos bsrc (Conversion.n2i npos1) (Conversion.n2i nsz) btgt  (Conversion.n2i npos2)
+   ".
+
+Extract Constant BufferPlain.copy_sz_pos =>
+   "
+    fun bsrc npos1 nsz btgt npos2 -> Conversion.i2n @@
+      Mlcpp_cstdio.Cstdio.File.Buffer.copy_sz_pos bsrc (Conversion.n2i npos1) (Conversion.n2i nsz) btgt  (Conversion.n2i npos2)
+   ".
+
+Extract Constant cpp_store_chunk_to_path =>
+   "
+    fun fp nsz npos b -> Conversion.i2n @@
+      Helper.store_chunk_to_path (Mlcpp_filesystem.Filesystem.Path.from_string fp) (Conversion.n2i nsz) (Conversion.n2i npos) b
+   ".
+
+Extract Constant cpp_load_chunk_from_path =>
+   "
+    fun fp -> Helper.load_chunk_from_path (Mlcpp_filesystem.Filesystem.Path.from_string fp)
+   ".
+
+
+(* extract into "lxr.ml" all named modules and definitions, and their dependencies *)
+Extraction "lxr.ml"  Conversion Utilities Configuration Buffer RelationAidKey RelationFileAid Assembly.
