theories/RelationAidKey.v
@@ -1,0 +1,43 @@
+(**
+      e L y K s e e R
+*)
+
+From LXR Require Import Rel.
+
+Module Export RelationAidKey <: REL.
+
+(**
+ Module: RelationAidKey
+ Description: relates assembly to key
+ *)
+
+From Coq Require Import Strings.String NArith PArith FMaps.
+Open Scope string_scope.
+
+Module Import M := FMapList.Make(String_as_OT).
+(* Print M. *)
+
+Record keyinformation : Type := mkkeyinformation
+    { pkey : string
+    }.
+
+Definition key := M.key.
+
+Definition elt := keyinformation.
+
+Definition Map : Type := M.t elt.
+
+Definition new : Map := M.empty _.
+
+Definition find (name : key) (rel : Map) : option elt := M.find name rel.
+
+Definition add (name : key) (bi : elt) (rel : Map) : Map := M.add name bi rel.
+
+Section Tests.
+
+Definition rel1 := (add "none" {|pkey:="empty"|} (add "abc97391af" {| pkey := "guessme" |} new)).
+Compute find "abc97391af" rel1.
+
+End Tests.
+
+End RelationAidKey.
