theories/RelationFileAid.v
@@ -1,0 +1,53 @@
+(**
+      e L y K s e e R
+*)
+
+From LXR Require Import Rel.
+
+Module Export RelationFileAid <: REL.
+
+(**
+ Module: RelationFileAid
+ Description: relates file names to assembly
+ *)
+
+From Coq Require Import Strings.String NArith PArith FMaps.
+Open Scope string_scope.
+
+Module Import M := FMapList.Make(String_as_OT).
+(* Print M. *)
+
+Record blockinformation : Type := mkblockinformation
+    { blockid : positive
+    ; bchecksum : string
+    ; blocksize : N
+    ; filepos : N
+    ; blockaid : string
+    ; blockapos : N
+    }.
+
+Definition key := M.key.
+
+Definition elt := list blockinformation.
+
+Definition Map : Type := M.t elt.
+
+Definition new : Map := M.empty _.
+
+Definition find (name : key) (rel : Map) : option elt := M.find name rel.
+
+Definition add (name : key) (bis : elt) (rel : Map) : Map :=
+    (* let entries :=
+        match M.find name rel with
+        | Some bis => bi :: bis
+        | None => bi :: nil
+        end in *)
+     M.add name bis rel.
+
+Section Tests.
+
+Compute find "test.txt" (add "test.txt" ({| blockid := 1; bchecksum := "chk"; blocksize := 37; filepos := 0; blockaid := "abc97391af"; blockapos := 0 |} :: nil) new).
+
+End Tests.
+
+End RelationFileAid.
