theories/Rel.v
@@ -1,0 +1,11 @@
+
+(* this is the signature for relations *)
+
+Module Type REL.
+    Parameter key : Type.
+    Parameter elt : Type.
+    Parameter Map : Type.
+    Parameter new : Map.
+    Parameter find : key -> Map -> option elt.
+    Parameter add : key -> elt -> Map -> Map.
+End REL.
